WIP: simulate consistency step

src/mapping/RMWPromising.v
@@ -374,6 +374,23 @@ Section RMWLocal.
       unfold proj_sumbool in x0. des_ifs. congr.
   Qed.
 
+  Variant fulfillable_ts (ts: Time.t) (lc: Local.t (A:=A)) (mem: Memory.t): Prop :=
+    | fulfillable_ts_intro
+        (LT_VWN: lt lc.(Local.vwn).(View.ts) ts)
+        (LT_VCAP: lt lc.(Local.vcap).(View.ts) ts)
+  .
+
+  Lemma fulfillable_ts_le
+        ts lc1 lc2 mem
+        (LC_LE: Local.le lc1 lc2)
+        (FULFILLABLE: fulfillable_ts ts lc2 mem):
+    fulfillable_ts ts lc1 mem.
+  Proof.
+    inv FULFILLABLE. econs.
+    - eapply Nat.le_lt_trans; [|exact LT_VWN]. apply LC_LE.
+    - eapply Nat.le_lt_trans; [|exact LT_VCAP]. apply LC_LE.
+  Qed.
+
   Definition fulfillable (lc: Local.t (A:=A)) (mem: Memory.t): Prop :=
     forall ts (PROMISED: Promises.lookup ts lc.(Local.promises) = true),
       (<<LT_VWN: lt lc.(Local.vwn).(View.ts) ts>>) /\
